***NO_CI*** WIP; getting the wp proof to go through for a toy example

examples/seplogic/Lang.fst
@@ -8,6 +8,7 @@ open FStar.ST
 open FStar.Heap  //this order of opening the modules is important, we want ref from FStar.Heap
 
 open FStar.Tactics
+open FStar.Tactics.Logic
 
 type addr = ref int
 
@@ -36,23 +37,29 @@ assume val interpreted_in (#a:Type0) (c:command a) (h:heap) :Tot (a * heap)
 
 type heap_predicate = heap -> Type0
 
-let is_emp (h:heap) : Type0 = (h == emp)
+let is_emp (h:heap) : Type0 = (equal h emp)
 
 let points_to (id:addr) (n:int) (h:heap) :Type0 =
-  (h == (restrict h (Set.singleton (addr_of id)))) /\ (sel h id == n)
-
+  (equal h (restrict h (Set.singleton (addr_of id)))) /\ (sel h id == n)
+    
 let lift (phi:Type0) (h:heap) :Type0 = phi /\ is_emp h
 
 let exists_x (#a:Type0) (pred:a -> heap_predicate) (h:heap) :Type0
   = exists (x:a). pred x h
 
 let star (p:heap_predicate) (q:heap_predicate) (h:heap) :Type0
-  = exists (h1:heap) (h2:heap). disjoint h1 h2 /\ (h == (join h1 h2)) /\ p h1 /\ q h2
+  = exists (h1:heap) (h2:heap). disjoint h1 h2 /\ (equal h (join h1 h2)) /\ p h1 /\ q h2
 
 let iff (p:heap_predicate) (q:heap_predicate) :Type0 = forall (h:heap). p h <==> q h
 
 let imp (p:heap_predicate) (q:heap_predicate) :Type0 = forall (h:heap). p h ==> q h
 
+let restrict_r (h:heap) (r:addr) : GTot heap
+  = restrict h (Set.singleton (addr_of r))
+
+let exclude_r (h:heap) (r:addr) : GTot heap
+  = exclude h (Set.singleton (addr_of r))
+  
 type c_pre            = heap_predicate
 type c_post (a:Type0) = a -> heap_predicate
 
@@ -74,48 +81,96 @@ type hoare_triple (#a:Type0) (pre:c_pre) (c:command a) (post:c_post a)
 
 let rec wpsep_command (#a:Type0) (c:command a) :st_wp a
   = match c with
-    | Return #a x      -> fun p h0 -> h0 == emp /\ p x h0
+    | Return #a x      -> fun p h0 -> (equal h0 emp) /\ p x h0
 
     | Bind #a #b c1 c2 ->
       FStar.Classical.forall_intro (FStar.WellFounded.axiom1 #a #(command b) c2);
-      fun p h3 -> exists (h2' h2'':heap). h3 ==  h2' `join` h2'' /\
-                                  (wpsep_command c1) (fun x h1 -> exists h1' h1''. h1' `join` h1'' == h1 `join` h2'' /\
+      fun p h3 -> exists (h2' h2'':heap). h3 `equal` (h2' `join` h2'') /\
+                                  (wpsep_command c1) (fun x h1 -> exists h1' h1''. (h1' `join` h1'') `equal` (h1 `join` h2'') /\
 						                           (wpsep_command (c2 x)) (fun y h2 -> p y (h2 `join` h1'')) h1') h2'      
 
     | Read r    -> fun p h0 -> (exists x. points_to r x h0) /\ (forall x. points_to r x h0 ==> p x h0)
 
     | Write r y -> fun p h0 -> (exists x. points_to r x h0) /\ (forall h1. points_to r y h1 ==> p () h1)
 
-    | Alloc     -> fun p h0 -> h0 == emp /\ (forall r h1. points_to r 0 h1 ==> p r h1)
+    | Alloc     -> fun p h0 -> (equal h0 emp) /\ (forall r h1. points_to r 0 h1 ==> p r h1)
 
 let lift_wpsep (#a:Type0) (wp_sep:st_wp a) :st_wp a
-  = fun p h0 -> exists h0' h0''. h0 == h0' `join` h0'' /\
+  = fun p h0 -> exists h0' h0''. h0 `equal` (h0' `join` h0'') /\
                          wp_sep (fun x h1' -> p x (h1' `join` h0'')) h0'
 
-let rec lift_command (#a:Type0) (c:command a) :st_wp a
-  = match c with
-    | Return #a x        -> fun p h0 ->  p x h0
+// let rec lift_command (#a:Type0) (c:command a) :st_wp a
+//   = match c with
+//     | Return #a x        -> fun p h0 ->  p x h0
     
-    | Bind #a #b c1 c2   ->    
-       FStar.Classical.forall_intro (FStar.WellFounded.axiom1 #a #(command b) c2);
-       fun p h0 -> exists h0' h0''. h0 == h0' `join` h0'' /\
-                            (lift_command c1) (fun x h1 -> lift_command (c2 x)  (fun x h2 -> p x (h2 `join` h0''))  h1)  h0' 
+//     | Bind #a #b c1 c2   ->    
+//        FStar.Classical.forall_intro (FStar.WellFounded.axiom1 #a #(command b) c2);
+//        fun p h0 -> exists h0' h0''. h0 == h0' `join` h0'' /\
+//                             (lift_command c1) (fun x h1 -> lift_command (c2 x)  (fun x h2 -> p x (h2 `join` h0''))  h1)  h0' 
  
-    | Read r    -> fun p h0 -> let h0' = restrict h0 (Set.singleton (addr_of r)) in
-                             exists h0''. h0 == h0' `join` h0'' /\
-                             (exists x. points_to r x h0') /\ (forall x. points_to r x h0'  ==>  p x (h0' `join` h0''))
+//     | Read r    -> fun p h0 -> let h0' = restrict h0 (Set.singleton (addr_of r)) in
+//                              exists h0''. h0 == h0' `join` h0'' /\
+//                              (exists x. points_to r x h0') /\ (forall x. points_to r x h0'  ==>  p x (h0' `join` h0''))
 					    
-    | Write r y -> fun p h0 -> let h0' = restrict h0 (Set.singleton (addr_of r)) in
-                             exists h0''. h0 == h0' `join` h0'' /\
-                             (exists x. points_to r x h0') /\ (forall h1. points_to r y h1 ==> p () (h1 `join` h0''))  
+//     | Write r y -> fun p h0 -> let h0' = restrict h0 (Set.singleton (addr_of r)) in
+//                              exists h0''. h0 == h0' `join` h0'' /\
+//                              (exists x. points_to r x h0') /\ (forall h1. points_to r y h1 ==> p () (h1 `join` h0''))  
 					   
-    | Alloc     -> fun p h0 -> (forall r h1. points_to r 0 h1 ==> p r (h1 `join` h0)) 
+//     | Alloc     -> fun p h0 -> (forall r h1. points_to r 0 h1 ==> p r (h1 `join` h0)) 
+
+
+// let lemma_ret_alloc_helper (h:heap) (phi: heap -> heap -> prop)
+//   :Lemma (phi emp h ==> (exists (h':heap) (h'':heap). h == h' `join` h'' /\ h' == emp /\ phi h' h''))
+//   = ()
+
+// let lemma_return_alloc (u:unit)
+//   :Lemma (forall (h:heap) (phi: heap -> heap -> prop).
+// 	 (phi emp h ==> (exists (h':heap) (h'':heap). h == h' `join` h'' /\ h' == emp /\ phi h' h'')))
+//   = FStar.Classical.forall_intro_2 lemma_ret_alloc_helper
+				   
+// let lemma_read (h:heap) (r:addr) (phi:int -> heap -> heap -> prop)
+//   :Lemma (requires (exists x. points_to r x (restrict_r h r) ) /\
+//                             (forall y. points_to r y (restrict_r h r) ==> phi y (restrict_r h r) (exclude_r h r)))
+//               (ensures (exists h' h''. h == h' `join` h'' /\
+// 	         (exists x. points_to r x h') /\ (forall y. points_to r y h' ==> phi y h' h'')))
+//   = lemma_join_restrict_exclude h (Set.singleton (addr_of r))
+
+// let lemma_write (h:heap) (r:addr) (y:int) (phi:heap -> heap -> prop)
+//   :Lemma (requires (exists x. points_to r x (restrict_r h r)) /\
+//                             ((forall h1. points_to r y h1 ==> phi h1 (exclude_r h r))))
+//               (ensures (exists (h':heap) (h'':heap). h == h' `join` h'' /\  
+// 	          ((exists x. points_to r x h') /\ (forall h1. points_to r y h1 ==> phi h1 h''))))
+//   = lemma_join_restrict_exclude h (Set.singleton (addr_of r))	      
+//
+// let lemma_split_h_emp (h:heap) (phi:heap -> heap -> prop)
+//   :Lemma (requires phi h emp)
+//                  (ensures (exists (h':heap) (h'':heap). h == h' `join` h'' /\ phi h' h''))
+//   = ()
+
+let lemma_read_write (phi:heap -> heap -> prop) (r:addr) (h:heap)
+  :Lemma (requires (exists x. points_to r x (restrict_r h r)) /\ phi (restrict_r h r) (exclude_r h r))
+              (ensures (exists h1 h2. h `equal` (h1 `join` h2) /\ ((exists x. points_to r x h1) /\ phi h1 h2)))
+  = lemma_join_restrict_exclude h (Set.singleton (addr_of r))
+
+let lemma_restrict_points_to (phi:prop) (r:addr) (h:heap{h `contains` r})
+  :Lemma (requires phi)
+              (ensures (exists x. points_to r x (restrict_r h r)) /\ phi)
+  = ()
+
+let lemma_select_excluded_join (x:int) (r:addr) (h1:heap) (h2:heap)
+  :Lemma (requires sel h1 r == x)
+              (ensures sel (h1 `join` (exclude_r h2 r)) r == x)
+  = admit()
+
+let lemma_points_to (h:heap) (r:addr) (x:int)
+  :Lemma (requires points_to r x h)
+              (ensures sel h r  == x)
+  = ()
 
 let steps :list step = [delta_only
   ["Lang.wp_command";
    "Lang.wpsep_command";
    "Lang.lift_wpsep";
-   "Lang.lift_command";
    "Lang.disjoint_partitions";
    "Lang.uu___is_Return";
    "Lang.uu___is_Bind";
@@ -137,7 +192,7 @@ let steps :list step = [delta_only
 #reset-options "--z3rlimit 5"
 
 let unfold_fns :list string = [
-  "wp_command"; "wpsep_command"; "lift_wpsep"; "lift_command"; "disjoint_partitions"; "uu___is_Return"; "uu___is_Bind";
+  "wp_command"; "wpsep_command"; "lift_wpsep"; "disjoint_partitions"; "uu___is_Return"; "uu___is_Bind";
   "uu___is_Read"; "uu___is_Write"; "uu___is_Alloc"; "__proj__Return__item__v";
    "__proj__Bind__item__c1"; "__proj__Bind__item__c2"; "__proj__Read__item__id";
    "__proj__Write__item__id"; "__proj__Write__item__v"
@@ -146,12 +201,21 @@ let unfold_fns :list string = [
 unfold let unfold_steps =
   List.Tot.map (fun s -> pack_fv ["Lang"; s]) unfold_fns
 
-let foo (r1:addr) (r2:addr) (h:heap{sel h r2 == 4 /\ addr_of r1 <> addr_of r2})
-  = let c = Bind (Write r1 3) (fun _ -> Read r1) in
-    let p :st_post int = fun _ h -> sel h r2 == 4 in
-(*    let t = (lift_wpsep (wpsep_command c)) p h in *)
-    let t = (lift_command c) p h in
-    assert_by_tactic t (norm [Delta; UnfoldOnly unfold_steps; Primops];; dump "Foo")
+let foo (r1:addr) (r2:addr) (h:heap{h `contains` r1})
+  = let c = (Write r1 3) in
+    let p = fun _ h -> sel h r1 == 3 in
+    let t = (lift_wpsep (wpsep_command c)) p h in 
+    assert_by_tactic t (norm [Delta; UnfoldOnly unfold_steps; Primops];; 
+                              apply_lemma (quote (lemma_read_write));;
+                              apply_lemma (quote (lemma_restrict_points_to));; 
+                              norm[Simpl];;			      
+                              forall_intro;;
+                              implies_intro;;	
+                              apply_lemma (quote (lemma_select_excluded_join));;
+                              norm[Simpl];;
+                              apply_lemma (quote (lemma_points_to));;
+	            smt;;
+                              dump "Foo")
 
 
 // exists h0' h0''. h == h0' `join` h0'' /\
